Basics of cache unlock operation
Spec is a bit tricky: want to cacheI in pre/post condition so that
caller can call unlock several times and then prove on their own that
publishing these values is ok. Tricky part is ensuring that the spec
proves all the cache parts of the obligation, so caller can just prove
the rest of Inv and R.

src/ConcurrentCache2.v
@@ -792,4 +792,90 @@ Proof.
   eauto.
 Admitted.
 
+Definition unlock {T} a rx : prog _ _ T :=
+  tid <- GetTID;
+  l <- Get MLocks;
+  let l' := set_open l a in
+  Assgn MLocks l';;
+  GhostUpdate (fun s =>
+    let l := get GLocks s in
+    let l' := free_lock l a in
+    let vd := get GDisk s in
+    let vd' := lin_release vd tid a in
+    let vd0 := get GDisk0 s in
+    let vd0' := match vd (a, Owned tid) with
+                | Some (v, _) => upd vd0 a v
+                | None => vd0
+                end in
+    set GDisk0 vd0'
+      (set GDisk vd'
+      (set GLocks l' s)));;
+  rx tt.
+
+Hint Rewrite get_free_lock using (solve [ auto ] ) : locks.
+Hint Rewrite get_free_lock_other using (solve [ auto ] ) : locks.
+
+Theorem linearized_consistent_free : forall V (m: @linear_mem addr _ V)
+  locks a tid,
+  linearized_consistent m (Locks.get locks) ->
+  linearized_consistent (lin_release m tid a) (Locks.get (free_lock locks a)).
+Proof.
+  unfold linearized_consistent, lin_release; intros.
+  specialize (H a0).
+  destruct (weq a a0); subst;
+    autorewrite with locks; intros; cbn;
+    destruct matches.
+Qed.
+
+Hint Resolve linearized_consistent_free.
+
+Theorem unlock_ok : forall a,
+    stateS TID: tid |-
+    {{ Fs F F0 LF vd0 vd v v0,
+     | PRE d m s0 s:
+         hlistmem s |= Fs * haddr GDisk0 |-> vd0 * rep vd /\
+         Inv m s d /\
+         vd |= F * lin_pred (Owned tid) (cache_locked tid s (LF * a |-> (v, None))) /\
+         vd0 |= F0 * a |-> v0 /\
+         R tid s0 s
+     | POST d' m' s0' s' _:
+        exists vd0' vd',
+           hlistmem s' |= Fs * haddr GDisk0 |-> vd0' * rep vd' /\
+           Inv m' s' d' /\
+           vd' |= F * (a, NoOwner) |-> (v, None) *
+             lin_pred (Owned tid) (cache_locked tid s LF) /\
+           vd0' |= F0 * a |-> v /\
+           s0' = s0
+    }} unlock a.
+Proof.
+  hoare pre simplify with try solve [ finish ].
+  eapply cache_rep_refold; eauto.
+
+  unfold pred_in.
+  rewrite hlistupd_memupd.
+  rotate_left.
+  rotate_left.
+  eapply ptsto_upd'.
+  rewrite hlistupd_memupd.
+  rotate_right.
+  rotate_right.
+  eapply ptsto_upd'.
+  rewrite hlistupd_memupd.
+  rotate_right.
+  eapply ptsto_upd'.
+  rotate_left.
+  eauto.
+
+  finish.
+  unfold cacheI; repeat descend; autorewrite with hlist; eauto.
+  admit.
+  admit.
+
+  admit. (* cache_rep after lin_release *)
+  admit. (* important: GDisk0 has been updated at a *)
+
+  (* oops, can't promise Inv holds *)
+  give_up.
+Abort.
+
 End Cache.
